Add Default.v

src/GPUCSL/GPUCSL.v
@@ -6,5 +6,5 @@ Set Implicit Arguments.
 Unset Strict Implicit.
 
 Require Import MyVector.
-Definition default ntrd : (Vector.t assn ntrd * Vector.t assn ntrd) := 
+Definition defaultSpec ntrd : (Vector.t assn ntrd * Vector.t assn ntrd) := 
   (init (fun _ => Emp_assn), init (fun _ => Emp_assn)).
