src/Utils/Default.v
@@ -1,0 +1,10 @@
+Require Import PHeap List.
+
+Class hasDefval A := HD {default : A}.
+Global Instance Z_hasDefval : hasDefval Z := {default := 0%Z}.
+Global Instance val_hasDefval : hasDefval val := {default := VZ 0%Z}.
+Global Instance listA_hasDefval A : hasDefval (list A) := {default := nil}.
+Global Instance option_hasDefval A : hasDefval (option A) := {default := None}.
+Notation get ls i := (nth i ls default).
+Eval compute in get (1 :: 2 :: 3 :: nil)%Z 2.
+Eval compute in get (Some 1 :: Some 2 :: Some 3 :: nil)%Z 4.
